beginning to bidirectionalize val interp subst lemma

theories/iris/logrel/instr/typing/inst.v
@@ -131,6 +131,22 @@ Section inst.
       shred_for_up_mini ιss H02.
   Qed.
 
+  (* wow that was much easier than I thought it'd be *)
+  Lemma eval_rep_mem_irrel_eq se ρ μ :
+    eval_rep se ρ =
+    eval_rep (senv_insert_mem (Σ:=Σ) μ se) ρ.
+  Proof.
+    induction ρ using rep_ind; auto.
+    - cbn in *.
+      assert (H': mapM (eval_rep se) ρs = mapM (eval_rep (senv_insert_mem μ se)) ρs)
+        by by apply Forall_mapM_ext.
+      by rewrite H'.
+    - cbn in *.
+      assert (H': mapM (eval_rep se) ρs = mapM (eval_rep (senv_insert_mem μ se)) ρs)
+        by by apply Forall_mapM_ext.
+      by rewrite H'.
+  Qed.
+
   Lemma eval_rep_size_irrel se ρ ιs n :
     eval_rep se ρ = Some ιs ->
     eval_rep (senv_insert_size (Σ:=Σ) n se) ρ = Some ιs.
@@ -145,6 +161,21 @@ Section inst.
       shred_for_up_mini ιss H02.
   Qed.
 
+  Lemma eval_rep_size_irrel_eq se ρ n :
+    eval_rep se ρ =
+    eval_rep (senv_insert_size (Σ:=Σ) n se) ρ.
+  Proof.
+    induction ρ using rep_ind; auto.
+    - cbn in *.
+      assert (H': mapM (eval_rep se) ρs = mapM (eval_rep (senv_insert_size n se)) ρs)
+        by by apply Forall_mapM_ext.
+      by rewrite H'.
+    - cbn in *.
+      assert (H': mapM (eval_rep se) ρs = mapM (eval_rep (senv_insert_size n se)) ρs)
+        by by apply Forall_mapM_ext.
+      by rewrite H'.
+  Qed.
+
   Lemma eval_rep_type_irrel se ρ ιs sκ T :
     eval_rep se ρ = Some ιs ->
     eval_rep (senv_insert_type (Σ:=Σ) sκ T se) ρ = Some ιs.
@@ -157,6 +188,21 @@ Section inst.
     - cbn in *.
       apply fmap_Some in H0 as (ιss & H02 & ->).
       shred_for_up_mini ιss H02.
+  Qed.
+
+  Lemma eval_rep_type_irrel_eq se ρ sκ T :
+    eval_rep se ρ =
+    eval_rep (senv_insert_type (Σ:=Σ) sκ T se) ρ.
+  Proof.
+    induction ρ using rep_ind; auto.
+    - cbn in *.
+      assert (H': mapM (eval_rep se) ρs = mapM (eval_rep (senv_insert_type sκ T se)) ρs)
+        by by apply Forall_mapM_ext.
+      by rewrite H'.
+    - cbn in *.
+      assert (H': mapM (eval_rep se) ρs = mapM (eval_rep (senv_insert_type sκ T se)) ρs)
+        by by apply Forall_mapM_ext.
+      by rewrite H'.
   Qed.
 
   Lemma eval_size_mem_irrel se σ n μ :
@@ -178,6 +224,24 @@ Section inst.
       by apply eval_rep_mem_irrel.
   Qed.
 
+  Lemma eval_size_mem_irrel_eq se σ μ :
+    eval_size se σ =
+    eval_size (senv_insert_mem (Σ:=Σ) μ se) σ.
+  Proof.
+    induction σ using size_ind; intros; auto.
+    - cbn in *.
+      assert (H': mapM (eval_size se) σs = mapM (eval_size (senv_insert_mem μ se)) σs)
+        by by apply Forall_mapM_ext.
+      by rewrite H'.
+    - cbn in *.
+      assert (H': mapM (eval_size se) σs = mapM (eval_size (senv_insert_mem μ se)) σs)
+        by by apply Forall_mapM_ext.
+      by rewrite H'.
+    - Opaque senv_insert_mem.
+      cbn.
+      by rewrite <- eval_rep_mem_irrel_eq.
+  Qed.
+
   Lemma eval_size_type_irrel se σ n sκ T :
     eval_size se σ = Some n ->
     eval_size (senv_insert_type (Σ:=Σ) sκ T se) σ = Some n.
@@ -197,6 +261,24 @@ Section inst.
       by apply eval_rep_type_irrel.
   Qed.
 
+  Lemma eval_size_type_irrel_eq se σ sκ T :
+    eval_size se σ =
+    eval_size (senv_insert_type (Σ:=Σ) sκ T se) σ.
+  Proof.
+    induction σ using size_ind; intros; auto.
+    - cbn in *.
+      assert (H': mapM (eval_size se) σs = mapM (eval_size (senv_insert_type sκ T se)) σs)
+        by by apply Forall_mapM_ext.
+      by rewrite H'.
+    - cbn in *.
+      assert (H': mapM (eval_size se) σs = mapM (eval_size (senv_insert_type sκ T se)) σs)
+        by by apply Forall_mapM_ext.
+      by rewrite H'.
+    - Opaque senv_insert_type.
+      cbn.
+      by rewrite <- eval_rep_type_irrel_eq.
+  Qed.
+
   Lemma eval_kind_mem_irrel se κ sκ μ :
     eval_kind se κ = Some sκ ->
     eval_kind (senv_insert_mem (Σ:=Σ) μ se) κ = Some sκ.
@@ -211,6 +293,15 @@ Section inst.
       apply fmap_Some.
       pose proof (eval_size_mem_irrel _ _ _ μ H02).
       rewrite H. eexists; split; done.
+  Qed.
+
+  Lemma eval_kind_mem_irrel_eq se κ μ :
+    eval_kind se κ =
+    eval_kind (senv_insert_mem (Σ:=Σ) μ se) κ .
+  Proof.
+    destruct κ; intros; cbn in *.
+    - by rewrite <- eval_rep_mem_irrel_eq.
+    - by rewrite <- eval_size_mem_irrel_eq.
   Qed.
 
   Lemma eval_kind_type_irrel se κ sκ sκ' T :
@@ -229,6 +320,15 @@ Section inst.
       rewrite H. eexists; split; done.
   Qed.
 
+  Lemma eval_kind_type_irrel_eq se κ sκ T :
+    eval_kind se κ =
+    eval_kind (senv_insert_type (Σ:=Σ) sκ T se) κ .
+  Proof.
+    destruct κ; intros; cbn in *.
+    - by rewrite <- eval_rep_type_irrel_eq.
+    - by rewrite <- eval_size_type_irrel_eq.
+  Qed.
+
   Lemma type_skind_mem_irrel se μ τ sκ :
     type_skind (Σ:=Σ) se τ = Some sκ ->
     type_skind (Σ:=Σ) (senv_insert_mem μ se)
@@ -241,6 +341,18 @@ Section inst.
     all: rewrite rinstId'_kind.
     all: unfold eval_kind in *.
     all: by apply eval_kind_mem_irrel.
+  Qed.
+
+  Lemma type_skind_mem_irrel_eq se μ τ :
+    type_skind (Σ:=Σ) se τ =
+    type_skind (Σ:=Σ) (senv_insert_mem μ se)
+      (ren_type unscoped.shift unscoped.id unscoped.id unscoped.id τ).
+  Proof.
+    destruct τ.
+    1: done.
+    all: intros; cbn in *.
+    all: rewrite rinstId'_kind.
+    all: by apply eval_kind_mem_irrel_eq.
   Qed.
 
   Lemma eval_rep_up_rep se sub_r ιs0 i ιs :
@@ -409,6 +521,190 @@ Section inst.
     all: try (by apply eval_kind_type_irrel).
   Qed.
 
+  Lemma type_interp_eq_r τ se sv :
+    type_interp rti sr τ se sv -∗ (add_skind_interp τ $ pre_type_interp rti sr τ) se sv.
+  Proof.
+    iDestruct (type_interp_eq rti sr τ se sv) as "[help _]".
+    done.
+  Qed.
+
+  Lemma type_interp_eq_l τ se sv :
+    (add_skind_interp τ $ pre_type_interp rti sr τ) se sv -∗
+    type_interp rti sr τ se sv.
+  Proof.
+    iDestruct (type_interp_eq rti sr τ se sv) as "[_ help]".
+    done.
+  Qed.
+
+  (* seems fine, but omg we'll have to do All of them.... all four....
+     probably a decent amount of overlap but this is just so annoying
+   *)
+  Lemma type_interp_up_memory se sub_t μ sv i :
+    type_interp rti sr (sub_t i) se sv ∗-∗
+    type_interp rti sr (up_memory_type sub_t i) (senv_insert_mem μ se) sv.
+  Proof.
+    asimpl'.
+    unfold core.funcomp.
+    generalize dependent se.
+    generalize dependent sv.
+    induction (sub_t i) using type_ind with
+      (P0 := λ ft, ∀ cl se, closure_interp rti sr ft se cl ∗-∗
+        closure_interp rti sr (ren_function_type unscoped.shift unscoped.id unscoped.id unscoped.id ft)
+                               (senv_insert_mem μ se) cl).
+    1: { (* vart *)
+      intros; iSplitL; iIntros; cbn; done.
+    }
+    1: (* numbers *) {
+      intros; iSplitL; iIntros "H"; cbn.
+      all: iDestruct "H" as "(%sκ & %h1 & %h2 & h4)".
+      all: iExists sκ; iFrame.
+      all: iPureIntro.
+      all: split; try done.
+      - rewrite rinstId'_kind; by rewrite <- eval_kind_mem_irrel_eq.
+      - rewrite rinstId'_kind in h1. by rewrite <- eval_kind_mem_irrel_eq in h1.
+    }
+    1: admit. (* should be the same as numbers *)
+    1: { (* sum *)
+      (* iIntros (?) "H"; cbn. *)
+      (* iDestruct "H" as "(%sκ & %h1 & h2 & h4)". *)
+      (* iExists sκ; iFrame. *)
+      (* iSplitR; rewrite rinstId'_kind; [iPureIntro; by apply eval_kind_mem_irrel|]. *)
+      (* cbn in H. *)
+      (* okay yes it's forall stuffs *)
+      admit.
+    }
+
+    4: { (* reft *)
+      intros. iSplitL; iIntros "H";
+        iPoseProof (type_interp_eq_r with "[$H]") as "H";
+        iApply type_interp_eq_l;
+        iDestruct "H" as "(%sκ & %h1 & h2 & h4)";
+        iExists sκ; iFrame;
+        [ iSplitR; [iPureIntro; by rewrite <- type_skind_mem_irrel_eq|]
+        | iSplitR; [iPureIntro; by rewrite <- type_skind_mem_irrel_eq in h1|]].
+      {
+        (* now to figure out how to use the IH *)
+        cbn.
+        assert (eval_mem_up_shift_mem: eval_mem se m =
+                                         eval_mem (senv_insert_mem μ se) (ren_memory unscoped.shift m)
+               ). {
+          admit.
+        }
+        rewrite eval_mem_up_shift_mem.
+        destruct (eval_mem (senv_insert_mem μ se) (ren_memory unscoped.shift m)) eqn:h.
+        2: rewrite h; cbn; done.
+        rewrite h; cbn.
+        destruct b.
+        - (* memmm *)
+          cbn.
+          iDestruct "h4" as "(%ℓ & %fs & %ws & #h1 & h2 & h3 & h4)".
+          iExists ℓ, fs, ws.
+          iFrame "∗".
+          iSplitR; auto.
+          iModIntro.
+          by iApply IHo.
+        - (* memgc *)
+          cbn.
+          iDestruct "h4" as "(%ℓ & %fs & h1 & hinv)".
+          iExists ℓ, fs. iFrame.
+          iApply (na_inv_iff with "[$] [-]").
+          repeat iModIntro.
+          iSplitR; iIntros "H".
+          all: iDestruct "H" as "(%ws & h1 & h2 & h3)".
+          all: iExists ws; iFrame.
+          all: iModIntro.
+          all: by iApply IHo.
+      }
+      {
+        cbn.
+        assert (eval_mem_up_shift_mem: eval_mem se m =
+                                         eval_mem (senv_insert_mem μ se) (ren_memory unscoped.shift m)
+               ). {
+          admit.
+        }
+        rewrite eval_mem_up_shift_mem.
+        destruct (eval_mem (senv_insert_mem μ se) (ren_memory unscoped.shift m)) eqn:h.
+        2: rewrite h; cbn; done.
+        rewrite h; cbn.
+        destruct b.
+        - (* memmm *)
+          cbn.
+          iDestruct "h4" as "(%ℓ & %fs & %ws & #h1 & h2 & h3 & h4)".
+          iExists ℓ, fs, ws.
+          iFrame "∗".
+          iSplitR; auto.
+          iModIntro.
+          by iApply IHo.
+        - (* memgc *)
+          cbn.
+          iDestruct "h4" as "(%ℓ & %fs & h1 & hinv)".
+          iExists ℓ, fs. iFrame.
+          iApply (na_inv_iff with "[$] [-]").
+          repeat iModIntro.
+          iSplitR; iIntros "H".
+          all: iDestruct "H" as "(%ws & h1 & h2 & h3)".
+          all: iExists ws; iFrame.
+          all: iModIntro.
+          all: by iApply IHo.
+      }
+    }
+
+    4: { (* codereft, test of the inductive hypothesis *)
+      intros; iSplitL; iIntros "H";
+        iPoseProof (type_interp_eq_r with "[$H]") as "H";
+        iApply type_interp_eq_l;
+        iDestruct "H" as "(%sκ & %h1 & h2 & h4)";
+        iExists sκ; iFrame;
+        [ iSplitR; [iPureIntro; by rewrite <- type_skind_mem_irrel_eq|]
+        | iSplitR; [iPureIntro; by rewrite <- type_skind_mem_irrel_eq in h1|]].
+      all: cbn.
+      all: iDestruct "h4" as "(%i0 & %i32 & %j & %cl & h1 & h2 & h3 & h4)".
+      all: iExists i0, i32, j, cl.
+      all: iFrame.
+      all: by iApply IHo.
+    }
+
+    8: { (* exists mem *)
+      intros; iSplitL; iIntros "H";
+        iPoseProof (type_interp_eq_r with "[$H]") as "H";
+        iApply type_interp_eq_l;
+        iDestruct "H" as "(%sκ & %h1 & h2 & h4)";
+        iExists sκ; iFrame;
+        [ iSplitR; [iPureIntro; by rewrite <- type_skind_mem_irrel_eq|]
+        | iSplitR; [iPureIntro; by rewrite <- type_skind_mem_irrel_eq in h1|]].
+      Transparent senv_insert_mem.
+      all: cbn in *.
+      {
+        asimpl'.
+        (* okay I think this is true but this looks really damn annoying to prove *)
+        admit.
+      }
+      {
+        admit.
+      }
+    }
+
+    11: { (* monofun, base case of inductive hyp *)
+      intros; iSplitL; iIntros "H".
+      {
+        assert (H': closure_interp rti sr (MonoFunT τs1 τs2) se cl -∗
+               mono_closure_interp rti sr τs1 τs2
+                  (map (type_interp rti sr) τs1) (map (type_interp rti sr) τs2) se cl). {
+          iIntros "H"; iApply "H".
+        }
+        iPoseProof (H' with "[$H]") as "H".
+        unfold mono_closure_interp.
+        (* okay staring at it seems doable *)
+        admit.
+      }
+      {
+        admit.
+      }
+
+
+    }
+
+  Admitted.
 
   (** STARTING FROM HERE, we begin to have these assumptions about how substitutions and semantic envs
       relate to one another. These relations are strong enough to prove the necessary subsitution
@@ -435,7 +731,21 @@ Section inst.
     by apply H in Hlookup as (H0 & _).
   Qed.
 
-  Ltac unfold_sem_rels := unfold sem_env_rel_rep, sem_env_rel_size, sem_env_rel_type, sem_env_rel_sκ in *.
+  Definition sem_env_rel_rep_eq (se' : @semantic_env Σ) (se : @semantic_env Σ) (sub_r:nat → representation) :=
+    (forall i, lookup_rep se' i = eval_rep se (sub_r i)).
+  Definition sem_env_rel_size_eq (se' : @semantic_env Σ) (se : @semantic_env Σ) (sub_s:nat → Core.size) :=
+    (forall i, lookup_size se' i = eval_size se (sub_s i)).
+  Definition sem_env_rel_type_eq_BAD (se' : @semantic_env Σ) (se : @semantic_env Σ) (sub_t:nat → type) :=
+    (forall i sκ' T', lookup_type se' i = Some (sκ', T') ->
+    type_skind se (sub_t i) = Some sκ' /\
+      (∀ sv, (T' sv -∗ ⌜skind_has_svalue sκ' sv⌝ -∗ value_interp rti sr se (sub_t i) sv))).
+  Definition sem_env_rel_sκ_eq (se' : @semantic_env Σ) (se : @semantic_env Σ) (sub_t:nat → type) :=
+    (forall i, fst <$> lookup_type se' i =
+    type_skind se (sub_t i)).
+
+
+  Ltac unfold_sem_rels := unfold sem_env_rel_rep, sem_env_rel_size, sem_env_rel_type, sem_env_rel_sκ,
+    sem_env_rel_rep_eq, sem_env_rel_size_eq, sem_env_rel_type_eq_BAD, sem_env_rel_sκ_eq in *.
 
 
 
@@ -457,6 +767,30 @@ Section inst.
       shred_for_up ιss Hρs.
     - intros ??; cbn in *; done.
   Qed.
+
+  Lemma eval_rep_subst_senv_eq (se se' : semantic_env (Σ:=Σ)) sub_r ρ :
+    sem_env_rel_rep_eq se' se sub_r ->
+    eval_rep se' ρ =
+    eval_rep se (subst_representation sub_r ρ).
+  Proof.
+    intros Hsub_r; unfold_sem_rels.
+    induction ρ as [n|ρs IH|ρs IH|ιs'] using rep_ind.
+    - cbn in *. by apply Hsub_r.
+    - cbn.
+      assert (H': mapM (eval_rep se') ρs = mapM (eval_rep se) (map (subst_representation sub_r) ρs)). {
+        apply Forall2_mapM_ext.
+        (* yes this is true by IH *)
+        admit.
+      }
+      by rewrite H'.
+    - cbn.
+      assert (H': mapM (eval_rep se') ρs = mapM (eval_rep se) (map (subst_representation sub_r) ρs)). {
+        apply Forall2_mapM_ext.
+        admit.
+      }
+      by rewrite H'.
+    - cbn in *; done.
+  Admitted.
 
   Lemma eval_size_subst_env (se se' : semantic_env (Σ:=Σ)) sub_r sub_s σ n :
     sem_env_rel_rep se' se sub_r ->
@@ -624,117 +958,74 @@ Section inst.
       admit.
   Admitted.
 
-  Lemma type_interp_eq_r τ se sv :
-    type_interp rti sr τ se sv -∗ (add_skind_interp τ $ pre_type_interp rti sr τ) se sv.
-  Proof.
-    iDestruct (type_interp_eq rti sr τ se sv) as "[help _]".
-    done.
-  Qed.
-
-  Lemma type_interp_eq_l τ se sv :
-    (add_skind_interp τ $ pre_type_interp rti sr τ) se sv -∗
-    type_interp rti sr τ se sv.
-  Proof.
-    iDestruct (type_interp_eq rti sr τ se sv) as "[_ help]".
-    done.
-  Qed.
-  (* As mentioned in a lower comment, this might require an additional assumption *)
-  (* this is also now safe from contamination :3 *)
-  Lemma values_interp_subst_type se se' τs os sub_m sub_r sub_s sub_t :
+  Lemma type_interp_subst_type_BIDIRECTIONAL se se' τ o sub_m sub_r sub_s sub_t :
     (sem_env_rel_rep se' se sub_r) ->
     (sem_env_rel_size se' se sub_s) ->
     (sem_env_rel_type se' se sub_t) ->
-    values_interp rti sr se' τs os -∗
-    values_interp rti sr se (map (subst_type sub_m sub_r sub_s sub_t) τs) os.
+    type_interp rti sr τ se' o ∗-∗
+    type_interp rti sr (subst_type sub_m sub_r sub_s sub_t τ) se o.
   Proof.
     iIntros (Hsub_r Hsub_s Hsub_T).
-    pose proof (rel_type_implies_rel_sκ se' se sub_t Hsub_T) as Hsub_t.
-    (* comment/uncomment if you want/dont' want to see them *)
+    (* pose proof (rel_type_implies_rel_sκ se' se sub_t Hsub_T) as Hsub_t. *)
+    (* comment/uncomment if you want/don't want to see them *)
     unfold_sem_rels.
-    generalize dependent os; generalize dependent τs.
-    induction τs as [| τ τs].
-    - intros os. iIntros "Hos". destruct os; done.
-    - intros os_big; iIntros "Hos".
-      cbn.
-      iDestruct "Hos" as "(%oss_big & %Hos_big & Hos)".
-      destruct oss_big as [|o oss]; [done|].
-      rewrite big_sepL2_cons.
-      rewrite big_sepL2_fmap_l.
-      iDestruct "Hos" as "[Hoa Hτsoss]".
-      cbn in IHτs.
-      setoid_rewrite big_sepL2_fmap_l in IHτs.
-      specialize (IHτs (concat oss)).
-      iDestruct IHτs as "#IHτs".
-      iAssert (∃ oss0, ⌜concat oss = concat oss0⌝ ∗
-            ([∗ list] τ0;os ∈ τs;oss0, value_interp rti sr se' τ0 (SAtoms os)))%I with "[Hτsoss]"
-        as "Hτs'". {
-        iExists oss; iSplitR; done.
+    generalize dependent o.
+    generalize dependent se'.
+    generalize dependent se.
+    generalize dependent sub_m.
+    generalize dependent sub_s.
+    generalize dependent sub_r.
+    generalize dependent sub_t.
+    generalize dependent τ.
+    induction τ using type_ind with
+      (P0 := λ ft, ∀ se se' cl sub_m sub_r sub_s sub_t,
+           sem_env_rel_rep se' se sub_r ->
+           sem_env_rel_size se' se sub_s ->
+           sem_env_rel_type se' se sub_t ->
+           closure_interp rti sr ft se' cl ∗-∗
+              closure_interp rti sr (subst_function_type sub_m sub_r sub_s sub_t ft) se cl).
+    * (** vart, qed *)
+      intros. cbn.
+      iSplitL.
+      {
+        iIntros "Hoa".
+        iDestruct "Hoa" as "(%sκ & %Hse'skind & Hoa & Htypevar)".
+        pose proof (rel_type_implies_rel_sκ se' se sub_t Hsub_T) as Hsub_t.
+        apply Hsub_t in Hse'skind as Htypeskind.
+        (* destruct Htypeskind as (sκ' & Htypeskind & Hsubsk). *)
+        (* inversion Hsubsk; subst. *)
+        destruct (se'.2 !! idx) eqn:Hse'typenv;
+          [| rewrite Hse'typenv in Hse'skind; cbn in Hse'skind; by inversion Hse'skind].
+        destruct o0 as [sκ' T].
+        assert (temp: sκ' = sκ). {
+          rewrite Hse'typenv in Hse'skind. cbn in Hse'skind. by inversion Hse'skind.
+        }
+        subst sκ'.
+
+        rewrite Hse'typenv.
+        iEval (cbn) in "Htypevar".
+
+
+        apply Hsub_T in Hse'typenv as [_ Hsub_T_true].
+        specialize (Hsub_T_true o).
+        unfold value_interp in Hsub_T_true.
+        iApply (Hsub_T_true with "[$] [$]").
       }
-      iPoseProof ("IHτs" with "[$Hτs']") as "Hτs''".
-      iDestruct "Hτs''" as "(%oss' & %Hc & Hτoss')".
-      (* note: concat oss = concat oss' does not simply oss = oss'. A bit stupid but okay. *)
-
-      iExists (o :: oss'); iSplitR. {
-        iPureIntro.
-        rewrite concat_cons; rewrite concat_cons in Hos_big. by rewrite <- Hc.
+      {
+        iIntros "Hoa".
+        admit.
       }
-      iApply big_sepL2_cons.
-      rewrite !big_sepL2_fmap_l.
-      iSplitL "Hoa"; first last.
-      + done.
-        (* I could have said first done but then there'd be so many bullets to change... *)
-      + (* this is where the fun begins *)
-        iClear "IHτs".
-        clear IHτs Hos_big Hc os_big oss τs Hsub_t.
-        (* I need it to not be SAtoms o. I'm scared. *)
-        (* generalize dependent o. *)
-        generalize dependent (SAtoms o).
-        generalize dependent se'.
-        generalize dependent se.
-        generalize dependent sub_m.
-        generalize dependent sub_s.
-        generalize dependent sub_r.
-        generalize dependent sub_t.
-        generalize dependent τ.
-        induction τ using type_ind with
-          (P0 := λ ft, ∀ se se' cl sub_m sub_r sub_s sub_t,
-               sem_env_rel_rep se' se sub_r ->
-               sem_env_rel_size se' se sub_s ->
-               sem_env_rel_type se' se sub_t ->
-               closure_interp rti sr ft se' cl -∗
-               closure_interp rti sr (subst_function_type sub_m sub_r sub_s sub_t ft) se cl).
-        * (** vart, do swords case *)
-          intros. cbn in *.
-          iDestruct "Hoa" as "(%sκ & %Hse'skind & Hoa & Htypevar)".
-          destruct sκ as [ιs ξ | n ξ]; [iDestruct "Hoa" as "[%Harep %Hflag]"
-                                       |iDestruct "Hoa" as "[%Hsizeinterp %Hflag]"].
-          2: admit. (* TODO *)
-          (* This is now using the correct Hsub_t *)
-          pose proof (rel_type_implies_rel_sκ se' se sub_t Hsub_T) as Hsub_t.
-          apply Hsub_t in Hse'skind as Htypeskind.
-          (* destruct Htypeskind as (sκ' & Htypeskind & Hsubsk). *)
-          (* inversion Hsubsk; subst. *)
-          destruct (se'.2 !! idx) eqn:Hse'typenv;
-            [| rewrite Hse'typenv in Hse'skind; cbn in Hse'skind; by inversion Hse'skind].
-          destruct o0 as [sκ' T].
-          assert (temp: sκ' = SVALTYPE ιs ξ). {
-            rewrite Hse'typenv in Hse'skind. cbn in Hse'skind. by inversion Hse'skind.
-          }
-          subst sκ'.
-
-          rewrite Hse'typenv.
-          iEval (cbn) in "Htypevar".
+      (*
+    * (* i31, qed *)
+      intros; cbn.
+      iDestruct "Hoa" as "(%sk & %HEval & %Hoa & _)".
+      iExists sk; iSplitR; [iPureIntro | iSplitR; [iPureIntro; done | done]].
+      by eapply eval_kind_subst_senv.
 
 
-          apply Hsub_T in Hse'typenv as [_ Hsub_T_true].
-          specialize (Hsub_T_true s).
-          iApply (Hsub_T_true with "[$] []").
-          iPureIntro; by split.
-        * (* i31, qed *)
-          intros; cbn.
-          iDestruct "Hoa" as "(%sk & %HEval & %Hoa & _)".
-          iExists sk; iSplitR; [iPureIntro | iSplitR; [iPureIntro; done | done]].
-          by eapply eval_kind_subst_senv.
+
+
+
         * (* numt, qed *)
           intros. cbn.
           iDestruct "Hoa" as "(%sk & %HEval & %Hoa & _)".
@@ -764,6 +1055,7 @@ Section inst.
           (* idk how to work with these maps but lemme get some of this out *)
           assert (H': ∃ τi, τs !! i = Some τi /\ τi_interp = type_interp rti sr τi). {
             (* obvious by Hτi_interp *)
+
             admit.
           }
           destruct H' as (τi & Hτi_lookup & Hτi).
@@ -784,6 +1076,7 @@ Section inst.
                            Some (type_interp rti sr (subst_type sub_m sub_r sub_s sub_t τi))).
                   {
                     (* this by τs !! i = Some τi *)
+
                     admit.
                   }
              by rewrite H'.
@@ -961,6 +1254,456 @@ Section inst.
              }
              apply Hsub_T in H' as (Hsκ0' & HT').
              split; [by apply type_skind_up_memory|].
+             iIntros (sv) "HT' #Hsv".
+             iPoseProof (HT' with "[$] [$]") as "Hval".
+             (* HERE *)
+             (* oh no...
+                need a lemma like
+                value_interp rti sr se (sub_t i) sv -∗
+                value_interp rti sr (senv_insert_mem μ se) (up_memory_type sub_t i) sv
+                and all the other combinations for all the other exists
+                jeez
+              *)
+             admit.
+        * (* exists rep *)
+          admit.
+        * (* exists size *)
+          admit.
+        * (* exists type *)
+
+          admit.
+        * (** MonoFun, WORRIED due to potential bi-implication *)
+          (* base case for P0 *)
+          iIntros (??????? Hsub_r Hsub_s Hsub_T) "#Hcl".
+          (* cbn. *)
+          (* I'm so scared *)
+          destruct cl; [|auto].
+          destruct f as [τs1_trans τs2_trans] eqn:Hf.
+          iDestruct "Hcl" as "(%Hτs1 & %Hτs2 & Hcl)".
+          iSplitR; [iPureIntro| iSplitR; [iPureIntro|]]; fold (subst_type sub_m sub_r sub_s sub_t).
+          -- pose proof (rel_type_implies_rel_sκ se' se sub_t Hsub_T) as Hsub_t.
+             by eapply translate_types_subst_senv.
+          -- pose proof (rel_type_implies_rel_sκ se' se sub_t Hsub_T) as Hsub_t.
+             by eapply translate_types_subst_senv.
+          -- iIntros "!> !> %%% Hvs Hos Hrt Hown Hfr Hrun".
+             iApply (cwp_label_wand with "[-]").
+             ++ iApply (cwp_return_wand with "[-]").
+                ** iApply (cwp_wand with "[-]").
+                   --- iApply ("Hcl" with "[$] [Hos] [$] [$] [$] [$]").
+                       iClear "Hcl".
+                       (* IT'S THE OTHER WAY AROUND WHYYYYY :SOB: *)
+                       admit. (* values_interp0 *)
+                   --- iClear "Hcl".
+                       iIntros (f' vs) "((%os & Hvs & Hos) & [% Hrt] & Hown)".
+                       iSplitL "Hvs Hos"; last iFrame.
+                       iExists _.
+                       iFrame.
+                       (* this is the correct direction to use H *)
+                       admit. (* values_interp0 *)
+                ** iClear "Hcl".
+                   iSplitL; first done.
+                   iIntros (? Hlen) "((% & Hvs & Hos) & [% Hrt] & Hown)".
+                   cbn in Hlen.
+                   iSplitL "Hvs Hos"; last iFrame.
+                   iExists _.
+                   iFrame.
+                   (* correct direction to use H0 *)
+                   admit. (* values_interp0 *)
+             ++ iClear "Hcl".
+                iSplitL; first done.
+                iApply big_sepL2_singleton.
+                iSplitL; first done.
+                iIntros (f' vs Hlen) "((% & Hvs & Hos) & [% Hrt] & Hown)".
+                cbn in Hlen.
+                iSplitL "Hvs Hos"; last iFrame.
+                iExists _.
+                iFrame.
+                (* correct direction to use H0 *)
+                admit.
+        * (* ForallMemT case, done except value interp mini lemma *)
+          intros ??????? Hsub_r Hsub_s Hsub_T.
+          iIntros "Hcl".
+          cbn.
+          iPoseProof "Hcl" as "#Hcl". (* to avoid cbn while in persistent *)
+          iModIntro.
+          iIntros.
+          iSpecialize ("Hcl" $! μ).
+          iApply IHτ; last done.
+          ++ intros ?? H'. asimpl'. apply eval_rep_mem_irrel. by apply Hsub_r.
+          ++ intros ?? H'. asimpl'.
+             apply eval_size_mem_irrel. by apply Hsub_s.
+          ++ intros ??? H'. asimpl'.
+             apply Hsub_T in H'.
+             destruct H' as [H1' H2'].
+             unfold core.funcomp.
+             split; [by apply type_skind_mem_irrel|].
+             (* this is going to be a value interp mem shifting thing *)
+             admit.
+        * (* ForallRepT *)
+          admit.
+        * (* ForallSizeT *)
+          intros ??????? Hsub_r Hsub_s Hsub_T.
+          admit.
+        * (* ForallTypeT *)
+          intros ??????? Hsub_r Hsub_s Hsub_T.
+          iIntros "Hcl"; cbn.
+          iDestruct "Hcl" as "(%sκ & %Hκ & Hcl)".
+          iExists sκ.
+          iSplitR; [iPureIntro; by eapply eval_kind_subst_senv|].
+          iIntros (?? Hsubs Hskind).
+          iSpecialize ("Hcl" $! sκ_T T Hsubs Hskind).
+          iPoseProof "Hcl" as "#Hcl".
+          iModIntro.
+
+          iApply IHτ; last done.
+          ++ intros ?? H'; asimpl'. unfold core.funcomp.
+             cbn in H'.
+             apply eval_rep_type_irrel.
+             by apply Hsub_r.
+          ++ intros ?? H'; asimpl'; unfold core.funcomp.
+             apply eval_size_type_irrel.
+             by apply Hsub_s.
+          ++ intros ??? H'.
+             cbn in H'.
+             destruct i.
+             -- cbn in *; inversion H'; subst.
+                split; [done|].
+                unfold unscoped.var_zero.
+                (* this is true *)
+                admit.
+             -- cbn in H'.
+                apply Hsub_T in H' as [H1' H2'].
+                split; [by apply type_skind_up_type|].
+                (* this is a value interp type shifting thing *)
+                admit.
+*)
+  Admitted.
+
+  (* As mentioned in a lower comment, this might require an additional assumption *)
+  (* this need to be a bimplication. Terrifying. *)
+  Lemma values_interp_subst_type se se' τs os sub_m sub_r sub_s sub_t :
+    (sem_env_rel_rep se' se sub_r) ->
+    (sem_env_rel_size se' se sub_s) ->
+    (sem_env_rel_type se' se sub_t) ->
+    values_interp rti sr se' τs os -∗
+    values_interp rti sr se (map (subst_type sub_m sub_r sub_s sub_t) τs) os.
+  Proof.
+    iIntros (Hsub_r Hsub_s Hsub_T).
+    pose proof (rel_type_implies_rel_sκ se' se sub_t Hsub_T) as Hsub_t.
+    (* comment/uncomment if you want/don't want to see them *)
+    unfold_sem_rels.
+    generalize dependent os; generalize dependent τs.
+    induction τs as [| τ τs].
+    - intros os. iIntros "Hos". destruct os; done.
+    - intros os_big; iIntros "Hos".
+      cbn.
+      iDestruct "Hos" as "(%oss_big & %Hos_big & Hos)".
+      destruct oss_big as [|o oss]; [done|].
+      rewrite big_sepL2_cons.
+      rewrite big_sepL2_fmap_l.
+      iDestruct "Hos" as "[Hoa Hτsoss]".
+      cbn in IHτs.
+      setoid_rewrite big_sepL2_fmap_l in IHτs.
+      specialize (IHτs (concat oss)).
+      iDestruct IHτs as "#IHτs".
+      iAssert (∃ oss0, ⌜concat oss = concat oss0⌝ ∗
+            ([∗ list] τ0;os ∈ τs;oss0, value_interp rti sr se' τ0 (SAtoms os)))%I with "[Hτsoss]"
+        as "Hτs'". {
+        iExists oss; iSplitR; done.
+      }
+      iPoseProof ("IHτs" with "[$Hτs']") as "Hτs''".
+      iDestruct "Hτs''" as "(%oss' & %Hc & Hτoss')".
+      (* note: concat oss = concat oss' does not imply oss = oss'. A bit stupid but okay. *)
+
+      iExists (o :: oss'); iSplitR. {
+        iPureIntro.
+        rewrite concat_cons; rewrite concat_cons in Hos_big. by rewrite <- Hc.
+      }
+      iApply big_sepL2_cons.
+      rewrite !big_sepL2_fmap_l.
+      iSplitL "Hoa"; first last.
+      + done.
+        (* I could have said first done but then there'd be so many bullets to change... *)
+      + (* this is where the fun begins *)
+        iClear "IHτs".
+        clear IHτs Hos_big Hc os_big oss τs Hsub_t.
+        (* I need it to not be SAtoms o. I'm scared. *)
+        (* it turned out okay :) *)
+        (* generalize dependent o. *)
+        generalize dependent (SAtoms o).
+        generalize dependent se'.
+        generalize dependent se.
+        generalize dependent sub_m.
+        generalize dependent sub_s.
+        generalize dependent sub_r.
+        generalize dependent sub_t.
+        generalize dependent τ.
+        induction τ using type_ind with
+          (P0 := λ ft, ∀ se se' cl sub_m sub_r sub_s sub_t,
+               sem_env_rel_rep se' se sub_r ->
+               sem_env_rel_size se' se sub_s ->
+               sem_env_rel_type se' se sub_t ->
+               closure_interp rti sr ft se' cl -∗
+               closure_interp rti sr (subst_function_type sub_m sub_r sub_s sub_t ft) se cl).
+        * (** vart, qed *)
+          intros. cbn in *.
+          iDestruct "Hoa" as "(%sκ & %Hse'skind & Hoa & Htypevar)".
+          (* This is now using the correct Hsub_t *)
+          pose proof (rel_type_implies_rel_sκ se' se sub_t Hsub_T) as Hsub_t.
+          apply Hsub_t in Hse'skind as Htypeskind.
+          (* destruct Htypeskind as (sκ' & Htypeskind & Hsubsk). *)
+          (* inversion Hsubsk; subst. *)
+          destruct (se'.2 !! idx) eqn:Hse'typenv;
+            [| rewrite Hse'typenv in Hse'skind; cbn in Hse'skind; by inversion Hse'skind].
+          destruct o0 as [sκ' T].
+          assert (temp: sκ' = sκ). {
+            rewrite Hse'typenv in Hse'skind. cbn in Hse'skind. by inversion Hse'skind.
+          }
+          subst sκ'.
+
+          rewrite Hse'typenv.
+          iEval (cbn) in "Htypevar".
+
+
+          apply Hsub_T in Hse'typenv as [_ Hsub_T_true].
+          specialize (Hsub_T_true s).
+          iApply (Hsub_T_true with "[$] [$]").
+        * (* i31, qed *)
+          intros; cbn.
+          iDestruct "Hoa" as "(%sk & %HEval & %Hoa & _)".
+          iExists sk; iSplitR; [iPureIntro | iSplitR; [iPureIntro; done | done]].
+          by eapply eval_kind_subst_senv.
+        * (* numt, qed *)
+          intros. cbn.
+          iDestruct "Hoa" as "(%sk & %HEval & %Hoa & _)".
+          iExists sk; iSplitR; [iPureIntro | iSplitR; [iPureIntro; done | done]].
+          by eapply eval_kind_subst_senv.
+        * (* sum, nearly qed except for map/forall2 lemmas *)
+          intros.
+          iPoseProof (type_interp_eq_r with "[$Hoa]") as "Hoa".
+          iApply type_interp_eq_l.
+          iDestruct "Hoa" as "(%sk & %HEval & %Hoa & Hsuminterp)".
+          iExists sk; iSplitR;
+            [iPureIntro; by eapply eval_kind_subst_senv |
+            iSplitR; [iPureIntro; done|]].
+          destruct κ as [ρ ξ|n ξ]; cbn in HEval;
+            apply bind_Some in HEval as (ιs & Hea & toinvert);
+            inversion toinvert; subst; cbn in Hoa; [|done]; clear toinvert.
+
+          destruct ρ; iEval (cbn) in "Hsuminterp"; try done.
+          rename l into ρs.
+
+          (* need to destruct Hsuminterp a bit more *)
+          iDestruct "Hsuminterp" as "(%i & %os & %off & %count &
+                              %H1 & %H2 & %H3 & Hoa)".
+          destruct (list_lookup i (map (type_interp rti sr) τs)) eqn:Hτi_interp; try done.
+          rename o0 into τi_interp.
+
+          (* idk how to work with these maps but lemme get some of this out *)
+          assert (H': ∃ τi, τs !! i = Some τi /\ τi_interp = type_interp rti sr τi). {
+            (* obvious by Hτi_interp *)
+
+            admit.
+          }
+          destruct H' as (τi & Hτi_lookup & Hτi).
+          subst τi_interp.
+
+          iExists i, os, off, count.
+
+          (* let's try to work with this now! *)
+          iSplitR; [done |
+            iSplitR; [iPureIntro |
+            iSplitR; [iPureIntro |]]]; last first.
+          -- pose proof (Forall_lookup_1 _ _ i τi H Hτi_lookup) as IH_τi.
+             specialize (IH_τi sub_t sub_r sub_s sub_m se se' Hsub_r Hsub_s Hsub_T
+                        (SAtoms (take count (drop off os)))).
+
+             assert (H': list_lookup i (map (type_interp rti sr)
+                              (map (subst_type sub_m sub_r sub_s sub_t) τs)) =
+                           Some (type_interp rti sr (subst_type sub_m sub_r sub_s sub_t τi))).
+                  {
+                    (* this by τs !! i = Some τi *)
+
+                    admit.
+                  }
+             by rewrite H'.
+          -- apply fmap_Some.
+             apply fmap_Some in H3 as (ιs_ρ & Hy & Hah).
+             exists ιs_ρ.
+             split; [|done].
+             apply bind_Some.
+             apply bind_Some in Hy as (ρ & Hz & Hbh).
+             cbn in Hbh.
+             exists (subst_representation sub_r ρ).
+             split.
+             ++ by apply map_lookup_helper.
+             ++ eapply eval_rep_subst_senv; done.
+          -- unfold sum_offset in *.
+             apply bind_Some in H2 as (ιss & Hy & Hah).
+             apply bind_Some.
+             (* hopefully *)
+             exists ιss. split; [|done].
+             (* Okay this is true by a combo of mapM lemmas and
+                eval_rep_subst_senv:
+                Hsub_r -> eval_rep se' ρ = Some ιs ->
+                eval_rep se (subst_representation sub_r ρ) = Some ιs
+              *)
+
+             apply mapM_Some.
+             apply mapM_Some in Hy.
+             (* seems a bit annoying to prove but definitely true:
+                - take i ρs and take i (map (..) ρs) operate on the same things
+                - On those things, use eval_rep_subst_senv, and you're good
+              *)
+             admit.
+        * (* variant qed except for map lemmas *)
+          intros.
+          iPoseProof (type_interp_eq_r with "[$Hoa]") as "Hoa".
+          iApply type_interp_eq_l.
+          iDestruct "Hoa" as "(%sκ & %Hsκ & %Hso & Hvariant)".
+
+          iExists sκ.
+          iSplitR; [iPureIntro; by eapply eval_kind_subst_senv|].
+          iSplitR; [done|].
+
+          iDestruct "Hvariant" as "(%i & %n & %ws & %ws' & %Hnat & %tosubst & Hoa)".
+          subst s.
+          destruct (list_lookup i (map (type_interp rti sr) τs)) eqn:Hτi_interp;
+            rewrite Hτi_interp; [|by cbn].
+          rename o0 into τi_interp.
+          assert (H': ∃ τi, τs !! i = Some τi /\ τi_interp = type_interp rti sr τi). {
+            (* obvious by Hτi_interp *)
+            admit.
+          }
+          destruct H' as (τi & Hτi_lookup & Hτi).
+          subst τi_interp.
+
+          iEval (cbn).
+          iExists i, n, ws, ws'.
+          iSplitR; [done | iSplitR; [done |]].
+          assert (H': list_lookup i (map (type_interp rti sr)
+                                       (map (subst_type sub_m sub_r sub_s sub_t) τs)) =
+                        Some (type_interp rti sr (subst_type sub_m sub_r sub_s sub_t τi))).
+          {
+            (* this by τs !! i = Some τi *)
+            admit.
+          }
+          rewrite H'.
+          pose proof (Forall_lookup_1 _ _ i τi H Hτi_lookup) as IH_τi.
+          by specialize (IH_τi sub_t sub_r sub_s sub_m se se' Hsub_r Hsub_s Hsub_T
+                        (SWords ws)).
+        * (* prod *)
+          admit.
+        * (* struct *)
+          admit.
+        * (** refT, induction fixed, now need varm relation and potential bidirectional *)
+          intros.
+          iPoseProof (type_interp_eq_r with "[$Hoa]") as "Hoa".
+          iDestruct "Hoa" as "(%sκ & %Hsκ & Hsκ & Hm)".
+          iApply type_interp_eq_l.
+          iExists sκ. (* used to destruct sκ first *)
+          iFrame.
+          iSplitR; [iPureIntro; by eapply eval_kind_subst_senv|].
+          (* huh. sure okay. I guess I don't need to have κ be valtype? *)
+          destruct m; [|destruct b].
+          --
+             (* I think this is where we now need some sort of varm relation? *)
+             (* interesting that before this was just done. Probably because of the
+                incorrect satoms *)
+             admit.
+          --
+             (* HWY IS IH\TAU SATOMS AAAAAAAAAA *)
+             (* is outdated :) no longer panic :) *)
+             iDestruct "Hm" as "(%ℓ & %fs & %ws & h1 & h2 & h3 & Hoa)".
+             iFrame.
+             iModIntro.
+             by eapply IHτ.
+          --
+             iDestruct "Hm" as "(%ℓ & %fs & h1 & Hinv)".
+             iFrame.
+             iExists fs.
+             (* I need some sort of "invariant implies another" *)
+             (* Search na_inv. *)
+             (* uh oh. na_inv_iff is similar. But. It's iff. *)
+             (* we only have one way. Uhoh. another place that requires bidirectional *)
+             (* Locate na_inv_iff. *)
+             (* hmmmmmmmmmmmmmmmmmmmmmmmmmmmmmmmmmmm TODO *)
+             admit.
+        * (* coderef, qed *)
+          (* I think this IH for function types is what we need but we'll see *)
+          intros.
+          iPoseProof (type_interp_eq_r with "[$Hoa]") as "Hoa".
+          iApply type_interp_eq_l.
+          iDestruct "Hoa" as "(%sκ & %Hsκ & Hsκ & (%i & %i32 & %j & %cl & Hcl))".
+          destruct sκ as [ιs ξ | n ξ]; [|].
+          2: { (* contradictory case, sκ = SMEMTYPE *)
+            iDestruct "Hcl" as "(_ & %tosubst & _)".
+            subst s.
+            iEval (cbn) in "Hsκ".
+            by iDestruct "Hsκ" as "[[]_]".
+          }
+          iExists (SVALTYPE ιs ξ).
+          iFrame.
+          iSplitR; [iPureIntro; by eapply eval_kind_subst_senv|].
+          iExists i, i32, j, cl.
+          iDestruct "Hcl" as "(H1 & H2 & H3 & H4 & H5)".
+          iFrame.
+          specialize (IHτ se se' cl sub_m sub_r sub_s sub_t Hsub_r Hsub_s Hsub_T).
+          iPoseProof IHτ as "IHτ".
+          by iApply IHτ.
+        * (* sert *)
+          admit.
+        * (* plug *)
+          admit.
+        * (* span *)
+          admit.
+        * (* rec *)
+          intros.
+
+          admit.
+        * (* exists mem, need mini value interp lemma, fix for memtype *)
+          intros.
+          iPoseProof (type_interp_eq_r with "[$Hoa]") as "Hoa".
+          iApply type_interp_eq_l.
+          iDestruct "Hoa" as "(%sκ & %Hsκ & Hsκ & (%μ & Hμ))".
+          iExists sκ.
+          iFrame. (* this does delete some pure things *)
+          iSplitR; [iPureIntro; eapply eval_kind_subst_senv; done|].
+
+          (* this might be wrong *)
+          cbn.
+          iExists μ.
+          iRename "Hμ" into "Hoa".
+
+          specialize (IHτ (up_memory_type sub_t) (up_memory_representation sub_r)
+                     (up_memory_size sub_s) (up_memory_memory sub_m))
+            as IHτ.
+          specialize (IHτ (senv_insert_mem μ se) (senv_insert_mem μ se'))
+            as IHτ.
+          apply IHτ.
+          -- intros.
+             assert (H': lookup_rep se' i = Some ιs'). {
+               unfold senv_insert_mem in H.
+               done.
+             }
+             apply Hsub_r in H'.
+             by apply eval_rep_up_memory.
+          -- intros.
+             assert (H': lookup_size se' i = Some n). {
+               cbn in H. done.
+             }
+             apply Hsub_s in H'.
+             by apply eval_size_up_memory.
+          -- intros.
+             assert (H': lookup_type se' i = Some (sκ', T')). {
+               unfold senv_insert_mem in H. cbn in H.
+               unfold lookup_type in *; cbn in H; by cbn.
+             }
+             apply Hsub_T in H' as (Hsκ0' & HT').
+             split; [by apply type_skind_up_memory|].
+             iIntros (sv) "HT' #Hsv".
+             iPoseProof (HT' with "[$] [$]") as "Hval".
+             (* HERE *)
              (* oh no...
                 need a lemma like
                 value_interp rti sr se (sub_t i) sv -∗
